specs/lemmas/Spec.Hash.Incremental.fst
@@ -16,10 +16,13 @@ open FStar.Mul
 module Loops = Lib.LoopCombinators
 
 /// A lemma I could not find in FStar.Math.Lemmas - note: duplicated in Hash.Streaming.Spec.fst
-let mul_zero_left_is_zero (n : nat) : Lemma(0 * n = 0) = ()
+let mul_zero_left_is_zero (n : int) : Lemma(0 * n = 0) = ()
+
+/// A lemma I could not find in FStar.Math.Lemmas - note: duplicated in Hash.Streaming.Spec.
+let mul_one_left_is_same (n : int) : Lemma(1 * n = n) = ()
 
 /// A lemma I could not find in FStar.Math.Lemmas
-let add_zero_right_is_same (n : nat) : Lemma(n + 0 = n) = ()
+let add_zero_right_is_same (n : int) : Lemma(n + 0 = n) = ()
 
 /// TODO: I don't find this lemma in Lib, and the below proofs don't work if
 /// I don't prove this step separately.
@@ -45,7 +48,7 @@ let update_multi_one_block_eq
      nat_to_extra_state a totlen'))) =
   let s = (hash, nat_to_extra_state a totlen) in
   let totlen' = nat_to_extra_state a (totlen + block_length a) in
-  extra_state_add_nat_bound_lem #a (nat_to_extra_state a totlen) (block_length a);
+  extra_state_add_nat_bound_lem1 #a (nat_to_extra_state a totlen) (block_length a);
   assert(totlen' == extra_state_add_nat #a (nat_to_extra_state a totlen) (block_length a));
   let block1, block2 = Lib.UpdateMulti.split_block (block_length a) block 1 in
   assert(block2 `S.equal` S.empty);
@@ -238,11 +241,8 @@ let blake2_no_finish
   (k : lbytes kk)
   (input : bytes {if kk = 0 then S.length input <= max_input_length a
                   else S.length input + block_length a <= max_input_length a}) =
-//  (input:bytes{Seq.length input <= max_input_length a}) =
   let nn = Blake2.max_output (to_blake_alg a) in
-//  let prev0 = Blake2.compute_prev0 (to_blake_alg a) 0 in
   let prev0 = Blake2.compute_prev0 (to_blake_alg a) kk in
-//  let s1 = Blake2.blake2_init (to_blake_alg a) 0 S.empty nn in
   let s1 = Blake2.blake2_init (to_blake_alg a) kk k nn in
   let (nb,rem) = Blake2.split (to_blake_alg a) (S.length input) in
   let s2 = Loops.repeati nb (Blake2.blake2_update1 (to_blake_alg a) prev0 input) s1 in
@@ -255,9 +255,7 @@ let blake2_hash_incremental_no_finish
   (k : lbytes kk)
   (input : bytes {if kk = 0 then S.length input <= max_input_length a
                   else S.length input + block_length a <= max_input_length a}) =
-//  (input:bytes{Seq.length input <= max_input_length a}) =
   let bs, l = split_blocks a input in
-//  let is1 = init a in
   let is1 = blake2_init a kk k in
   let is2 = update_multi a is1 bs in
   let is3 = update_last a is2 (S.length bs) l in
@@ -268,6 +266,304 @@ let blake2_hash_incremental_no_finish
 /// TODO: another weird thing: when I convert some asserts to asserts, the proof
 /// loops...
 /// TODO: the proof time is random
+
+let size_block_is_positive a :
+  Lemma(Spec.Blake2.size_block (to_blake_alg a) > 0) = ()
+
+let blake2_is_hash_incremental_aux1
+  (a:hash_alg{is_blake a})
+  (kk : size_nat{kk <= Blake2.max_key (to_blake_alg a)})
+  (k : lbytes kk)
+  (input : bytes {if kk = 0 then S.length input <= max_input_length a
+                  else S.length input + block_length a <= max_input_length a}) :
+  Lemma(
+    (**)
+    let nn = Spec.Blake2.max_output (to_blake_alg a) in
+    let prev0 = Blake2.compute_prev0 (to_blake_alg a) kk in
+    let s1 = Blake2.blake2_init (to_blake_alg a) kk k nn in
+    (**)
+    let bs, l = split_blocks a input in
+    let is1 = blake2_init a kk k in
+    ((s1 <: words_state' a), nat_to_extra_state a prev0) == is1) = ()
+
+/// Properties of the values returned by ``Spec.Blake2.split``
+let blake2_split_props (a:Blake2.alg) (len:nat) :
+  Lemma(
+    let nb, rem = Blake2.split a len in
+    rem <= len /\
+    rem <= Blake2.size_block a) = ()
+
+/// Properties of the values returned by ``split_blocks``. Note that ``split_blocks``
+/// has a postcondition which contains properties not duplicated here.
+/// TODO: might overlap ``split_at_last_num_blocks`` in Hacl.Streaming.Spec
+#push-options "--z3rlimit 100"
+let split_blocks_props (a:hash_alg{is_blake a}) (input:bytes) :
+  Lemma
+  (requires (S.length input <= max_input_length a))
+  (ensures (
+    let nb, rem = Blake2.split (to_blake_alg a) (S.length input) in
+    let bs, l = split_blocks a input in
+    Seq.length bs = nb * block_length a /\
+    Seq.length l = rem /\
+    rem <= block_length a /\
+    Seq.length input = Seq.length bs + rem /\
+    rem = Seq.length input - Seq.length bs /\ 
+    l `S.equal` S.slice input (S.length input - rem) (S.length input) /\
+    (Seq.length input <= block_length a ==>
+     (nb = 0 /\ rem = Seq.length input))))
+  = ()
+#pop-options
+
+/// Properties of the values return by ``last_split_blake``
+let last_split_blake_props (a:hash_alg{is_blake a}) (input : bytes) :
+  Lemma
+  (requires (Seq.length input <= block_length a))
+  (ensures (
+    let blocks, last_block, rem = last_split_blake a input in
+    blocks `Seq.equal` Seq.empty /\
+    rem = Seq.length input /\
+    last_block `Seq.equal` Blake2.get_last_padded_block (to_blake_alg a) input rem)) =
+  ()
+
+let last_split_blake_get_last_padded_block_eq (a:hash_alg{is_blake a}) (input : bytes) :
+  Lemma
+  (requires S.length input <= max_input_length a)
+  (ensures (
+    let nb, rem = Blake2.split (to_blake_alg a) (S.length input) in
+    let bs, l = split_blocks a input in
+    let last_block1 = Blake2.get_last_padded_block (to_blake_alg a) input rem in
+    let blocks, last_block2, rem = last_split_blake a l in
+    last_block2 `Seq.equal` last_block1)) =
+  let nb, rem = Blake2.split (to_blake_alg a) (S.length input) in
+  let bs, l = split_blocks a input in
+  let last_block1 = Blake2.get_last_padded_block (to_blake_alg a) input rem in
+  let blocks, last_block2, rem = last_split_blake a l in
+  assert(input `Seq.equal` Seq.append bs l);
+  blake2_split_props (to_blake_alg a) (S.length input);
+  split_blocks_props a input;
+  last_split_blake_props a l;
+  ()
+
+/// TODO: duplicate with Hacl.Streaming.Blake2s_32.fst
+/// TODO: move
+/// Equality between the state types defined by blake2s and the generic hash.
+/// The equality is not trivial because of subtleties linked to the way types are
+/// encoded for Z3.
+val state_types_equalities (a : hash_alg{is_blake a}) :
+  Lemma(Blake2.state (to_blake_alg a) == words_state' a)
+
+let state_types_equalities a =
+  let open Lib.Sequence in
+  let open Lib.IntTypes in
+  (* Because of the necessity to be able to normalize, we basically do
+   * the same proof twice. TODO: find a better way *)
+  match a with
+  | Blake2S ->
+    let a = Blake2S in (* small trick to get a proper normalization *)
+    let row = Blake2.row (to_blake_alg a) in
+    assert(Blake2.state (to_blake_alg a) == lseq row 4);
+    assert_norm(words_state' a == m:Seq.seq row {Seq.length m = 4});
+    assert_norm(lseq row 4 == m:Seq.seq row {Seq.length m == 4});
+    assert(lseq row 4 == m:Seq.seq row {Seq.length m = 4})
+  | Blake2B ->
+    let a = Blake2B in
+    let row = Blake2.row (to_blake_alg a) in
+    assert(Blake2.state (to_blake_alg a) == lseq row 4);
+    assert_norm(words_state' a == m:Seq.seq row {Seq.length m = 4});
+    assert_norm(lseq row 4 == m:Seq.seq row {Seq.length m == 4});
+    assert(lseq row 4 == m:Seq.seq row {Seq.length m = 4})
+
+let extra_state_v_nat_to_extra_state_is_id (a : hash_alg{is_blake a})
+                                           (n : nat{n <= max_extra_state a}) :
+  Lemma(extra_state_v (nat_to_extra_state a n) = n) = ()
+
+let compute_prev0_props (a:hash_alg{is_blake a}) (kk : nat) :
+  Lemma(
+    let prev0 = Blake2.compute_prev0 (to_blake_alg a) kk in
+    prev0 >= 0 /\
+    (if kk = 0 then prev0 = 0 else prev0 = block_length a)) = ()
+
+/// TODO: random time
+val blake2_is_hash_incremental_aux2
+  (a:hash_alg{is_blake a})
+  (kk : size_nat{kk <= Blake2.max_key (to_blake_alg a)})
+  (k : lbytes kk)
+  (input : bytes {if kk = 0 then S.length input <= max_input_length a
+                  else S.length input + block_length a <= max_input_length a})
+  (s1 : Blake2.state (to_blake_alg a)) :
+  Lemma(
+    let prev0 = Blake2.compute_prev0 (to_blake_alg a) kk in
+    let (nb,rem) = Blake2.split (to_blake_alg a) (S.length input) in
+    let s2 = Loops.repeati nb (Blake2.blake2_update1 (to_blake_alg a) prev0 input) s1 in
+    let bs, l = split_blocks a input in
+    let is2 = update_multi a (s1, nat_to_extra_state a prev0) bs in
+    s2 == fst is2)
+
+#push-options "--z3cliopt smt.arith.nl=false"
+let blake2_is_hash_incremental_aux2 a kk k input s1 =
+  assert_norm(Blake2.size_block (to_blake_alg a) = block_length a);
+  let prev0 = Blake2.compute_prev0 (to_blake_alg a) kk in
+  compute_prev0_props a kk;
+  let (nb,rem) = Blake2.split (to_blake_alg a) (S.length input) in
+  blake2_split_props (to_blake_alg a) (S.length input);
+  size_block_is_positive a;
+  assert(Spec.Blake2.size_block (to_blake_alg a) > 0);
+  assert(nb <= Seq.length input / Spec.Blake2.size_block (to_blake_alg a));
+  assert(prev0 <= block_length a);
+  assert(prev0 + Seq.length input <= Spec.Blake2.max_limb (to_blake_alg a));
+  let s2 = Loops.repeati #(Blake2.state (to_blake_alg a)) nb (Blake2.blake2_update1 (to_blake_alg a) prev0 input) s1 in
+  let bs, l = split_blocks a input in
+  split_blocks_props a input;
+  let is2 : words_state a = update_multi a (s1, nat_to_extra_state a prev0) bs in
+  assert(S.length bs == nb * block_length a);
+  assert(
+    nb * block_length a <= Seq.length input /\
+    prev0 + Seq.length input <= Blake2.max_limb (to_blake_alg a) /\
+    prev0 + nb * block_length a <= max_extra_state a);
+  repeati_blake2_update1_is_update_multi a nb prev0 input s1;
+  assert(
+    (Loops.repeati #(words_state' a) nb (Blake2.blake2_update1 (to_blake_alg a) prev0 input) s1,
+     nat_to_extra_state a (prev0 + nb * block_length a)) ==
+       update_multi a (s1, nat_to_extra_state a prev0) bs);
+  state_types_equalities a;
+  assert(words_state' a == Blake2.state (to_blake_alg a));
+  assert(((s2 <: words_state' a), nat_to_extra_state a (prev0 + nb * block_length a)) == is2)
+#pop-options
+
+(* TODO HERE
+#push-options "--z3cliopt smt.arith.nl=false"
+val blake2_is_hash_incremental_aux
+  (a:hash_alg{is_blake a})
+  (kk : size_nat{kk <= Blake2.max_key (to_blake_alg a)})
+  (k : lbytes kk)
+  (input : bytes {if kk = 0 then S.length input <= max_input_length a
+                  else S.length input + block_length a <= max_input_length a}) :
+  Lemma
+    (blake2_no_finish a kk k input == fst (blake2_hash_incremental_no_finish a kk k input))
+
+(* TODO HERE *)
+let blake2_is_hash_incremental_aux a kk k input =
+  assert_norm(Blake2.size_block (to_blake_alg a) = block_length a);
+  (* Let's prove the equality step by step *)
+  (* Introduce variables for the different steps of the left side of the equality *)
+  let nn = Spec.Blake2.max_output (to_blake_alg a) in
+  let prev0 = Blake2.compute_prev0 (to_blake_alg a) kk in
+  let s1 = Blake2.blake2_init (to_blake_alg a) kk k nn in
+  let nb, rem = Blake2.split (to_blake_alg a) (S.length input) in
+  mul_zero_left_is_zero (Blake2.size_block (to_blake_alg a));
+  assume(if kk = 0 then prev0 = 0 else prev0 = 1 * (Blake2.size_block (to_blake_alg a)));
+  Math.Lemmas.nat_times_nat_is_nat 1 (Blake2.size_block (to_blake_alg a));
+  assume(1 * (Blake2.size_block (to_blake_alg a)) >= 0);
+  assume(prev0 >= 0);
+  size_block_is_positive a;
+  assume(Spec.Blake2.size_block (to_blake_alg a) > 0);
+  assume(nb <= Seq.length input / Spec.Blake2.size_block (to_blake_alg a));
+  assume(prev0 + Seq.length input <= Spec.Blake2.max_limb (to_blake_alg a));
+  let s2 = Loops.repeati #(Blake2.state (to_blake_alg a)) nb (Blake2.blake2_update1 (to_blake_alg a) prev0 input) s1 in
+  assume(prev0 + Seq.length input <= Blake2.max_limb (to_blake_alg a));
+  blake2_split_props (to_blake_alg a) (S.length input);
+  assume(rem <= Seq.length input /\ rem <= Blake2.size_block (to_blake_alg a));
+  let s3 = Blake2.blake2_update_last (to_blake_alg a) prev0 rem input s2 in
+  (* Introduce variables for the different steps of the right side *)
+  let bs, l = split_blocks a input in
+  split_blocks_props a input;
+  let is1 : words_state a = blake2_init a kk k in
+  let is2 : words_state a = update_multi a is1 bs in
+  let is3 : words_state a = update_last a is2 (S.length bs) l in
+  (* Prove the equalities *)
+  (* [(s1, _) == is1] *)
+  assume(((s1 <: words_state' a), nat_to_extra_state a prev0) == is1);
+  (* [(s2, _) == is2] *)
+  assume(S.length bs == nb * block_length a); (* TODO: sometimes loops here - seems to have been fixed by ``split_blocks_props`` *)
+  assume(
+    nb * block_length a <= Seq.length input /\
+    prev0 + Seq.length input <= Blake2.max_limb (to_blake_alg a) /\
+    prev0 + nb * block_length a <= max_extra_state a);
+  repeati_blake2_update1_is_update_multi a nb prev0 input s1;
+  assume(
+    (Loops.repeati #(words_state' a) nb (Blake2.blake2_update1 (to_blake_alg a) prev0 input) s1,
+     nat_to_extra_state a (prev0 + nb * block_length a)) ==
+       update_multi a (s1, nat_to_extra_state a prev0) bs);
+  (* *)
+  state_types_equalities a;
+  assume(words_state' a == Blake2.state (to_blake_alg a));
+  assume(((s2 <: words_state' a), nat_to_extra_state a (prev0 + nb * block_length a)) == is2);
+  (* [s3 == fst is3] *)
+  (* First, work on [s3] *)
+  assume(rem == S.length input - S.length bs);
+  assume(l `S.equal` S.slice input (S.length input - rem) (S.length input));
+  let pblock = Blake2.get_last_padded_block (to_blake_alg a) input rem in
+  assume(
+    s3 == Blake2.blake2_update_block (to_blake_alg a) true (prev0 + S.length input) pblock s2);
+  (* Then, work on [is3] *)
+  assume(is3 == update_last_blake a is2 (S.length bs) l);
+  let blocks, last_block, rem' = last_split_blake a l in
+  last_split_blake_props a l;
+  last_split_blake_get_last_padded_block_eq a input;
+  assume(rem = rem');
+  assume(
+    blocks == S.empty /\
+    last_block == pblock /\
+    rem' = S.length l);
+  let h' : words_state a = update_multi a is2 S.empty in
+  update_multi_zero a is2;
+  assume(h' == is2);
+  assert_norm(max_input_length a == max_extra_state a);
+  assert(snd h' == nat_to_extra_state a (prev0 + S.length bs));
+  calc(==) {
+    extra_state_v (snd h');
+  (==) {}
+    extra_state_v (nat_to_extra_state a (prev0 + S.length bs));
+  (==) { extra_state_v_nat_to_extra_state_is_id a (prev0 + S.length bs) }
+    prev0 + S.length bs;
+  };
+  calc(==) {
+    extra_state_v (snd h') + rem;
+  (==) {}
+    (prev0 + S.length bs) + rem;
+  (==) { Math.Lemmas.paren_add_left prev0 (S.length bs) rem }
+    prev0 + S.length bs + rem;
+  (==) { Math.Lemmas.paren_add_right prev0 (S.length bs) rem }
+    prev0 + (S.length bs + rem);
+  (==) {}
+    prev0 + S.length input;
+  };
+  assert(extra_state_v (snd h') + rem <= max_extra_state a);
+
+  assert(rem <= max_extra_state a);
+  extra_state_add_nat_bound_lem2 #a (snd h') rem;
+  admit()
+
+(*
+  assert(extra_state_v (extra_state_add_nat (snd h') rem) ==
+         extra_state_v (nat_to_extra_state a ((extra_state_v (snd h')) + rem)));
+  admit()
+  calc (==) {
+    extra_state_v (extra_state_add_nat (snd h') rem);
+  (==) { extra_state_add_nat_bound_lem2 #a (snd h') rem }
+    extra_state_v (nat_to_extra_state a ((extra_state_v (snd h')) + rem));
+  (==) {}
+    extra_state_v (nat_to_extra_state a (prev0 + S.length input));
+  (==) { extra_state_v_nat_to_extra_state_is_id a (prev0 + S.length input) }
+    prev0 + S.length input;
+  };
+  admit()
+  extra_state_add_nat_bound_lem1 #a (snd h') rem;
+  admit()
+  (* TODO: above OK, fix below (proof seems to loop) *)
+  assert(extra_state_v (extra_state_add_nat (snd h') rem) == prev0 + S.length input);
+  assert(
+    is3 ==
+    (Spec.Blake2.blake2_update_block (to_blake_alg a) true
+                                     (extra_state_v (extra_state_add_nat (snd h') rem))
+                                     last_block (fst h'),
+     nat_to_extra_state a 0));
+  admit()
+  (* Prove the final equality *)
+  assert(s3 == fst is3)
+#pop-options
+
+(*
 #push-options "--z3rlimit 1000 --fuel 0 --ifuel 0"
 let blake2_is_hash_incremental_aux
   (a:hash_alg{is_blake a})
@@ -328,7 +624,7 @@ let blake2_is_hash_incremental_aux
   assert(max_input_length a == max_extra_state a);
   assert(snd h' == nat_to_extra_state a (prev0 + S.length bs));
   assert(extra_state_v (snd h') + rem == prev0 + S.length input);
-  extra_state_add_nat_bound_lem #a (snd h') rem;
+  extra_state_add_nat_bound_lem1 #a (snd h') rem;
   (* TODO: above OK, fix below (proof seems to loop) *)
   assert(extra_state_v (extra_state_add_nat (snd h') rem) == prev0 + S.length input);
   assert(
