specs/Spec.Hash.Lemmas.fsti
@@ -12,17 +12,22 @@ open Spec.Hash.PadFinish
 
 #set-options "--fuel 0 --ifuel 0 --z3rlimit 50"
 
-val extra_state_add_nat_bound_lem (#a:hash_alg{is_blake a}) (s : extra_state a)
-                                  (n:nat{n <= maxint (extra_state_int_type a)}) :
+val extra_state_add_nat_bound_lem1 (#a:hash_alg{is_blake a}) (s : extra_state a)
+                                  (n:nat{n <= max_extra_state a}) :
   Lemma
-  (requires extra_state_v s + n <= maxint (extra_state_int_type a))
-  (ensures extra_state_v (extra_state_add_nat s n) ==
-             extra_state_v s + n)
+  (requires extra_state_v s + n <= max_extra_state a)
+  (ensures extra_state_v (extra_state_add_nat s n) = extra_state_v s + n)
+
+val extra_state_add_nat_bound_lem2 (#a:hash_alg{is_blake a}) (s : extra_state a)
+                                  (n:nat{n <= max_extra_state a}) :
+  Lemma
+  (requires extra_state_v s + n <= max_extra_state a)
+  (ensures extra_state_add_nat s n == nat_to_extra_state a ((extra_state_v s) + n))
 
 val extra_state_add_nat_bound_associative_lem (#a:hash_alg{is_blake a}) (s : extra_state a)
                                               (n1 n2 : range_t (extra_state_int_type a)) :
   Lemma
-  (requires n1 + n2 <= maxint (extra_state_int_type a))
+  (requires n1 + n2 <= max_extra_state a)
   (ensures
        (extra_state_add_nat (extra_state_add_nat s n1) n2 ==
         extra_state_add_nat s (n1 + n2)))
